completeness: Truth lemma stub. Undone details left commented for now
Included in this commit is a proof of FormL.Elem being finite, i.e.
the existence of a surjection from Fin n to FormL.Elem.

This is useful for the applicative case of the Truth lemma.

Hybrid/Language/Context/Elem.lean
@@ -1,4 +1,4 @@
-import Hybrid.Language.Context
+import Hybrid.Language.Context.Def
 
 namespace FormL
 
@@ -10,6 +10,21 @@ namespace FormL
 -/
 def Elem {symbs : Symbols α} {sorts : List symbs.signature.S} (χ : FormL symbs sorts) :=
   (s : symbs.signature.S) × (φ : Form symbs s) × (φ.Context χ)
+
+@[simp]
+abbrev Elem.sort {symbs : Symbols α} {sorts : List symbs.signature.S} {χ : FormL symbs sorts} (e : χ.Elem) :=
+  e.1
+
+@[simp]
+abbrev Elem.form {symbs : Symbols α} {sorts : List symbs.signature.S} {χ : FormL symbs sorts} (e : χ.Elem) :=
+  e.2.1
+
+@[simp]
+abbrev Elem.ctx {symbs : Symbols α} {sorts : List symbs.signature.S} {χ : FormL symbs sorts} (e : χ.Elem) :=
+  e.2.2
+
+@[simp]
+abbrev num_forms : FormL symbs sorts → ℕ := λ _ => sorts.length
 
 /--
   Given a formula (list) `χ` and a natural number, will try to return the element in `χ` at the
@@ -45,7 +60,7 @@ def Context.toNat {φ : Form sig s} {χ : FormL sig sorts} : Context φ χ → �
 /--
   Any formula `χ` has a finite number of elements, so we can encode them to natural numbers.
 -/
-instance elem_encodable (χ : FormL symbs sorts) : Encodable χ.Elem where
+instance Elem.elem_encodable (χ : FormL symbs sorts) : Encodable χ.Elem where
   encode  := λ ⟨_, _, C⟩ => C.toNat
   decode  := χ.index
   encodek := by
@@ -61,3 +76,111 @@ instance elem_encodable (χ : FormL symbs sorts) : Encodable χ.Elem where
         rename_i ψ _ _
         simp [Context.toNat]
         simp [FormL.index, ih]
+
+lemma Elem.encode_wf {χ : FormL symbs sorts} : ∀ {e : χ.Elem}, Encodable.encode e < χ.num_forms := by
+  intro ⟨_, _, ctx⟩
+  induction χ with
+  | cons _ ψ _ ih =>
+      cases ctx with
+      | head => simp [Encodable.encode, num_forms, Context.toNat]
+      | tail ctx' =>
+          simp [Encodable.encode, num_forms, Context.toNat] at ih ⊢
+          apply ih
+  | _ =>
+      cases ctx
+      . simp [Encodable.encode, num_forms, Context.toNat]
+
+def get_elem (χ : FormL symbs sorts) : Fin χ.num_forms → χ.Elem
+  | ⟨0, _⟩ =>
+      match χ with
+      | @FormL.cons _ _ s _ _ ψ _ => ⟨s, ψ, .head⟩
+      | @FormL.prop _ _ s p       => ⟨s, .prop p, .refl⟩
+      | @FormL.nom _ _ s n        => ⟨s, .nom n, .refl⟩
+      | @FormL.svar _ _ s x       => ⟨s, .svar x, .refl⟩
+      | @FormL.appl _ _ _ _ rng σ φ => ⟨rng, .appl σ φ, .refl⟩
+      | @FormL.or _ _ s φ ψ       => ⟨s, .or φ ψ, .refl⟩
+      | @FormL.neg _ _ s φ        => ⟨s, .neg φ, .refl⟩
+      | @FormL.at _ _ _ s k φ     => ⟨s, .at k φ, .refl⟩
+      | @FormL.bind _ _ _ s x φ   => ⟨s, .bind x φ, .refl⟩
+  | ⟨n+1, lt⟩ =>
+        match χ with
+      | .cons _ ψ =>
+          let e := ψ.get_elem ⟨n, Nat.add_lt_add_iff_right.mp lt⟩
+          ⟨e.sort, e.form, .tail e.ctx⟩
+      | .prop _       => Nat.noConfusion $ Nat.lt_one_iff.mp lt
+      | .nom _        => Nat.noConfusion $ Nat.lt_one_iff.mp lt
+      | .svar _       => Nat.noConfusion $ Nat.lt_one_iff.mp lt
+      | .appl _ _     => Nat.noConfusion $ Nat.lt_one_iff.mp lt
+      | .or _ _       => Nat.noConfusion $ Nat.lt_one_iff.mp lt
+      | .neg _        => Nat.noConfusion $ Nat.lt_one_iff.mp lt
+      | .at _ _       => Nat.noConfusion $ Nat.lt_one_iff.mp lt
+      | .bind _ _     => Nat.noConfusion $ Nat.lt_one_iff.mp lt
+
+lemma get_elem_surj {χ : FormL symbs sorts} : χ.get_elem.Surjective := by
+  intro ⟨st, form, ctx⟩
+  let e : χ.Elem := ⟨st, form, ctx⟩
+  exists ⟨Encodable.encode e, Elem.encode_wf⟩
+  unfold e
+  clear e
+  induction χ with
+  | cons φ ψ _ ih =>
+      simp only [Encodable.encode]
+      cases ctx with
+      | head => simp only [Context.toNat, get_elem]
+      | tail ctx' =>
+          specialize ih ctx'
+          simp only [Encodable.encode] at ih
+          simp only [Context.toNat, get_elem, Elem.sort, Elem.form, Elem.ctx]
+          rw [ih]
+  | _ =>
+      simp only [Encodable.encode]
+      cases ctx
+      . simp! only [Fin.isValue, FormL.get_elem.eq_def]
+
+theorem Elem.enumerate {χ : FormL symbs sorts} {p : χ.Elem → Prop} : (∀ i : Fin χ.num_forms, p (χ.get_elem i)) ↔ (∀ e : χ.Elem, p e) := by
+  apply Iff.intro
+  . intro h e
+    have ⟨i, h_i⟩ := get_elem_surj e
+    rw [←h_i]
+    exact h i
+  . intro h i
+    exact h (χ.get_elem i)
+
+theorem Elem.enumerate' {χ : FormL symbs sorts} {p : {s : symbs.signature.S} → (φ : Form symbs s) → (φ.Context χ) → Prop} : (∀ i : Fin χ.num_forms, p (χ.get_elem i).form (χ.get_elem i).ctx) ↔ (∀ e : χ.Elem, p e.form e.ctx) := by
+  apply Iff.intro
+  . intro h e
+    have ⟨i, h_i⟩ := get_elem_surj e
+    rw [←h_i]
+    exact h i
+  . intro h i
+    exact h (χ.get_elem i)
+
+lemma Elem.sort_as_idx {ψ : FormL symbs sorts} {i : Fin ψ.num_forms} : (ψ.get_elem i).sort = sorts[i] := by
+  revert i
+  induction ψ with
+  | cons φ χ _ ih =>
+      simp only [List.length_cons, sort, Fin.getElem_fin]
+      rw [Fin.forall_fin_succ]
+      apply And.intro
+      . rename_i s₁ s₂ t a_ih
+        simp_all only [List.length_cons, List.length_nil, Nat.reduceAdd, sort, Fin.getElem_fin, Fin.val_eq_zero,
+          List.getElem_cons_zero, Fin.coe_ofNat_eq_mod, Nat.zero_mod]
+        obtain ⟨val, property⟩ := s₁
+        obtain ⟨val_1, property_1⟩ := s₂
+        rfl
+      . intro i
+        rename_i s₁ s₂ t a_ih
+        simp_all only [List.length_cons, List.length_nil, Nat.reduceAdd, sort, Fin.getElem_fin, Fin.val_eq_zero,
+          List.getElem_cons_zero, Fin.val_succ, List.getElem_cons_succ]
+        obtain ⟨val, property⟩ := s₁
+        obtain ⟨val_1, property_1⟩ := s₂
+        apply @ih
+  | _ =>
+      simp only [List.length_cons, List.length_nil, Nat.reduceAdd, sort, Fin.getElem_fin,
+        Fin.val_eq_zero, List.getElem_cons_zero]
+      intro i
+      cases i with
+      | mk val lt =>
+          simp only [Nat.lt_one_iff] at lt
+          subst lt
+          simp only [get_elem]
