Hybrid/Completeness/Henkin/Model.lean
@@ -10,27 +10,35 @@ variable [DecidableEq α]
 variable {symbs : Symbols α}
 variable {s t : symbs.signature.S}
 
+@[simp]
 abbrev NamedPastedWitnessedMCS.nominal_eq (Γ : NamedPastedWitnessedMCS symbs t Λ) (s : symbs.signature.S) (i j : symbs.nominal s) : Prop := ℋ@ i j ∈ Γ.set
 
-def nominal_eq.eqv {Γ : NamedPastedWitnessedMCS symbs t Λ} : Equivalence (Γ.nominal_eq s) where
-  refl := by
-    admit
-  symm := by
-    admit
-  trans := by
-    admit
+@[refl]
+abbrev NamedPastedWitnessedMCS.nominal_eq_refl (Γ : NamedPastedWitnessedMCS symbs t Λ) (s : symbs.signature.S) : ∀ (x : Symbols.nominal s), Γ.nominal_eq s x x := sorry
 
+@[symm]
+abbrev NamedPastedWitnessedMCS.nominal_eq_symm (Γ : NamedPastedWitnessedMCS symbs t Λ) (s : symbs.signature.S) : ∀ {x y : Symbols.nominal s}, Γ.nominal_eq s x y → Γ.nominal_eq s y x := sorry
+
+@[trans]
+abbrev NamedPastedWitnessedMCS.nominal_eq_trans (Γ : NamedPastedWitnessedMCS symbs t Λ) (s : symbs.signature.S) : ∀ {x y z : Symbols.nominal s}, Γ.nominal_eq s x y → Γ.nominal_eq s y z → Γ.nominal_eq s x z := sorry
+
+def nominal_eq.eqv {Γ : NamedPastedWitnessedMCS symbs t Λ} : Equivalence (Γ.nominal_eq s) where
+  refl := Γ.nominal_eq_refl s
+  symm := Γ.nominal_eq_symm s
+  trans := Γ.nominal_eq_trans s
+
+@[simp]
 instance NamedPastedWitnessedMCS.nominalSetoid (Γ : NamedPastedWitnessedMCS symbs t Λ) (s : symbs.signature.S) : Setoid (symbs.nominal s) where
   r := Γ.nominal_eq s
   iseqv := nominal_eq.eqv
 
-def WProd.to_args (Γ : NamedPastedWitnessedMCS symbs s Λ) : WProd symbs.nominal sorts → FormL symbs sorts :=
+def WProd.to_args : WProd symbs.nominal sorts → FormL symbs sorts :=
   match sorts with
   | []     => PEmpty.elim
   | _ :: t =>
       match t with
       | []     => λ i     => ℋNom i
-      | _ :: _ => λ i     => (ℋNom i.1).cons (to_args Γ i.2)
+      | _ :: _ => λ i     => (ℋNom i.1).cons (to_args i.2)
 
 def WProd.to_quotient (Γ : NamedPastedWitnessedMCS symbs s Λ) : WProd symbs.nominal sorts → WProd (λ s => Quotient (Γ.nominalSetoid s)) sorts :=
   match sorts with
@@ -40,13 +48,14 @@ def WProd.to_quotient (Γ : NamedPastedWitnessedMCS symbs s Λ) : WProd symbs.no
       | []     => λ i     => ⟦i⟧
       | _ :: _ => λ i     => ⟨⟦i.1⟧, to_quotient Γ i.2⟩
 
+@[simp]
 def NamedPastedWitnessedMCS.HenkinModel (Γ : NamedPastedWitnessedMCS symbs s Λ) : Model symbs where
   «Fr» := {
     W  := λ s => Quotient (Γ.nominalSetoid s),
     R  := λ {dom _} σ =>
         match dom with
         | [ ]    => { } -- constant σ case. TODO: make sure to support constant operators as formulas as well
-        | _ :: _ => { ⟨q, qs⟩ | ∃ j, ∃ (js : WProd symbs.nominal _), ℋ@ j (ℋ⟨σ⟩ (js.to_args Γ)) ∈ Γ.set ∧ (⟦j⟧ = q ∧ js.to_quotient Γ = qs) },
+        | _ :: _ => { ⟨q, qs⟩ | ∃ j, ∃ (js : WProd symbs.nominal _), ℋ@ j (ℋ⟨σ⟩ js.to_args) ∈ Γ.set ∧ (⟦j⟧ = q ∧ js.to_quotient Γ = qs) },
     Nm := λ n => ⟦.inl n⟧,
     WNonEmpty := λ s => ⟨⟦(symbs.signature.nNonEmpty s).default⟧⟩
   }
@@ -56,6 +65,45 @@ def NamedPastedWitnessedMCS.HenkinModel (Γ : NamedPastedWitnessedMCS symbs s Λ
 noncomputable def NamedPastedWitnessedMCS.HenkinAsgn (Γ : NamedPastedWitnessedMCS symbs s Λ) : Assignment Γ.HenkinModel :=
   λ x => ⟦Classical.choose $ Γ.witnessed.2 x⟧
 
-def nom_to_w (j : symbs.nominal t) (Γ : NamedPastedWitnessedMCS symbs s Λ) : Γ.HenkinModel.Fr.W t := ⟦j⟧
+lemma WProd.to_quotient_select {Γ : NamedPastedWitnessedMCS symbs s Λ} {φ : Form symbs t} {ψ : FormL symbs sorts} (ws : WProd symbs.nominal sorts) (C : φ.Context ψ) : (ws.to_quotient Γ).select C = ⟦ws.select C⟧ := by
+  admit
+
+lemma WProd.eq {ws ws' : WProd f ss} : ws = ws' ↔ ∀ {ψ : FormL symbs ss} {e : ψ.Elem}, ws.select e.ctx = ws'.select e.ctx := by
+  apply Iff.intro
+  . intros
+
+    admit
+  . intros
+    admit
+
+lemma WProd.to_quotient_eq_helper {Γ : NamedPastedWitnessedMCS symbs s Λ} {ws : WProd symbs.nominal sorts} {qs : WProd (λ s => Quotient (Γ.nominalSetoid s)) sorts} : ws.to_quotient Γ = qs ↔ ∀ {ψ : FormL symbs sorts} {e : ψ.Elem}, ⟦ws.select e.ctx⟧ = qs.select e.ctx := by
+  apply Iff.intro
+  . intro h ψ e
+    rw [←to_quotient_select]
+    rw [WProd.eq] at h
+    apply h
+  . rw [WProd.eq]
+    intro h ψ e
+    rw [to_quotient_select]
+    apply h
+
+lemma WProd.to_quotient_eq {Γ : NamedPastedWitnessedMCS symbs s Λ} {ws : WProd symbs.nominal sorts} {qs : WProd (λ s => Quotient (Γ.nominalSetoid s)) sorts} :
+  ws.to_quotient Γ = qs ↔
+  ∀ {ψ : FormL symbs sorts} {e : ψ.Elem}, ∃ j : symbs.nominal e.sort, ℋ@ j (ws.select e.ctx) ∈ Γ.set ∧ ⟦j⟧ = qs.select e.ctx := by
+  rw [to_quotient_eq_helper]
+  apply Iff.intro
+  . intro h ψ e
+    specialize @h ψ e
+    have ⟨j, h_rep⟩ := (qs.select e.ctx).exists_rep
+    simp only [NamedPastedWitnessedMCS.nominalSetoid, ← h_rep, Quotient.eq] at h
+    symm at h
+    exists j
+  . intro h ψ e
+    specialize @h ψ e
+    match h with
+    | ⟨j, ⟨h_equiv, h_rep⟩⟩ =>
+      simp only [NamedPastedWitnessedMCS.nominalSetoid, ← h_rep, Quotient.eq]
+      symm
+      exact h_equiv
 
 end Completeness
