Hybrid/Language/Context.lean
@@ -1,2 +1,3 @@
 import Hybrid.Language.Context.Def
+import Hybrid.Language.Context.Elem
 import Hybrid.Language.Context.Lemmas
